test.v
@@ -1,0 +1,16 @@
+From elpi Require Import elpi.
+
+Elpi Command B.
+Section A.
+  Context (A:Type).
+  Elpi Query  lp:{{
+    X = {{A}}
+  }}.
+  Elpi Accumulate  lp:{{
+    pred x i:term.
+    % x {{A}}. ERROR
+    x (global {{:gref A}}).
+  }}.
+  Elpi Typecheck.
+
+
